specIR/SIRProps.v
@@ -17,51 +17,520 @@ Require Import LinkingC.
 Require Import IntegersC.
 Require Import Mod ModSem Any Skeleton SimMod SimModSem.
 Require Import Sound SoundTop SimMem SimMemId SimSymb.
-Require Import SIRmini_quotient.
+Require Import SIRCommon2.
+Require Import SIRmini.
+Require Import SIRmini_stack.
+Require Import MatchSimModSemExcl.
 
 Require Import Program.
+Require Import SmallstepC.
 
 Set Implicit Arguments.
 
 
 
-Local Existing Instance SimMemOh_default.
-Global Arguments ModSemPair.mk [SM] [SS] _ _ _ _ [SMO].
+
+
+
+
+
+
+
+
+
+Import CatNotations.
+Open Scope cat_scope.
+
+
+
+
+
+
+
 
 Section OWNEDHEAP.
 
 Variable owned_heap: Type.
 Variable initial_owned_heap: SkEnv.t -> owned_heap.
+Variable mi: string.
+Variable prog: program owned_heap.
 
 
-Variable prog0 prog1: program owned_heap.
-Hypothesis TRANSL: 
 
 
 
+Section SMO.
+
+  Record t: Type :=
+    mk {
+      sm :> SimMem.t;
+      oh_src: Any;
+      oh_tgt: Any;
+    }
+  .
+
+  Inductive wf (smo: t): Prop :=
+  | wf_intro
+      (oh: owned_heap)
+      (MWF: SimMem.wf smo)
+      (OHSRC: smo.(oh_src) = upcast oh)
+      (OHTGT: smo.(oh_tgt) = upcast oh)
+  .
+
+  Local Obligation Tactic := try (by ii; des; ss).
+
+  Program Instance SimMemOh: (SimMemOh.class) :=
+    {|
+      SimMemOh.t := t;
+      SimMemOh.sm := sm;
+      SimMemOh.oh_src := oh_src;
+      SimMemOh.oh_tgt := oh_tgt;
+      SimMemOh.wf := wf;
+      SimMemOh.le := SimMem.le;
+      SimMemOh.lepriv := SimMem.lepriv;
+      SimMemOh.midx := Some mi;
+      SimMemOh.set_sm := fun smo sm => mk sm smo.(oh_src) smo.(oh_tgt);
+    |}
+  .
+  Next Obligation.
+    ii. eapply PR.
+  Qed.
+  Next Obligation.
+    ii. inv WF.
+    econs; ss; et.
+  Qed.
+  Next Obligation.
+    ss. ii. destruct smo0; ss.
+  Qed.
+
+End SMO.
 
 
 Section SIMMODSEM.
 
+Variable sk: Sk.t.
 Variable skenv_link: SkEnv.t.
 Variable sm_link: SimMem.t.
-Variable mi: string.
-Let md_src: Mod.t := (module prog0 mi initial_owned_heap).
-Let md_tgt: Mod.t := (module prog1 mi initial_owned_heap).
+Let md_src: Mod.t := (SIRmini.module sk prog mi initial_owned_heap).
+Let md_tgt: Mod.t := (SIRmini_stack.module sk prog mi initial_owned_heap).
+Let ms_src: ModSem.t := (Mod.modsem md_src skenv_link).
+Let ms_tgt: ModSem.t := (Mod.modsem md_tgt skenv_link).
 Hypothesis (INCLSRC: SkEnv.includes skenv_link (Mod.sk md_src)).
 Hypothesis (INCLTGT: SkEnv.includes skenv_link (Mod.sk md_tgt)).
 Hypothesis (WF: SkEnv.wf skenv_link).
 
+Local Existing Instance SimMemOh.
+Local Arguments ModSemPair.mk [SM] [SS] _ _ _ _ [SMO].
+
 Definition msp: ModSemPair.t := ModSemPair.mk (md_src skenv_link) (md_tgt skenv_link)
                                               (SimSymbId.mk md_src md_tgt) sm_link.
 
-Print SIR2.state.
-Print SIR3.state.
+Notation ktr :=
+  (ktree (eff1 owned_heap) (owned_heap * (mem * val)) (owned_heap * (mem * val)))
+.
+Notation itr := (itree (eff1 owned_heap) (owned_heap * (mem * val))).
 
-(* Theorem sim_modsem: ModSemPair.sim msp. *)
-(* Proof. *)
-(*   econs; eauto. *)
-(* Qed. *)
+Definition fold_cont (cont: list ktr): ktr :=
+  (* List.fold_left (fun s i => s >>> i) cont (id_ _) *)
+  List.fold_right (fun i s => i >>> s) (id_ _) cont
+.
+Hint Unfold fold_cont.
+
+(* Definition merge_events E R (itr: itree (E +' E) R): itree E R := *)
+(*   interp ((fun _ e => match e with *)
+(*                       | inl1 e => trigger e *)
+(*                       | inr1 e => trigger e *)
+(*                       end): ((E +' E) ~> itree E)) itr *)
+(* . *)
+(* Hint Unfold merge_events. *)
+
+(* Definition my_fix (itr1: (itree (eff1 owned_heap) (owned_heap * (mem * val)))): *)
+(*   (itree (eff0 owned_heap) (owned_heap * (mem * val))) := *)
+(*   merge_events (interp (bimap (interp_program0 prog) (id_ _)) itr1) *)
+(* . *)
+(* Hint Unfold my_fix. *)
+
+(* Definition my_fix (itr1: (itree (eff1 owned_heap) (owned_heap * (mem * val)))): *)
+(*   (itree (eff0 owned_heap) (owned_heap * (mem * val))) := *)
+(*   interp_mrec (interp_function prog) itr1 *)
+(* . *)
+(* Hint Unfold my_fix. *)
+
+
+
+
+Lemma eq_is_bisim: forall E R (t1 t2 : itree E R), t1 = t2 -> t1 ≅ t2.
+Proof. ii. clarify. reflexivity. Qed.
+Lemma bisim_is_eq: forall E R (t1 t2 : itree E R), t1 ≅ t2 -> t1 = t2.
+Proof. ii. eapply bisimulation_is_eq; eauto. Qed.
+
+Inductive match_states (idx: unit): SIRmini.state owned_heap ->
+          SIRmini_stack.state owned_heap -> SimMemOh.t -> Prop :=
+| match_states_intro
+    itr0 cur cont smo0
+    itr1
+    (FOLD: itr1 = (rvs <- cur ;; (fold_cont cont) rvs))
+    (SIM: itr0 = interp_mrec (interp_function prog) itr1)
+    (MWF: SimMemOh.wf smo0)
+    (SYNC: forall
+        oh0 m0 v0
+        (RET: itr0 = Ret (oh0, (m0, v0))),
+        <<OH: upcast oh0 = smo0.(SimMemOh.oh_src)>> /\ <<MEM: m0 = smo0.(SimMem.src)>>)
+  :
+    match_states idx itr0 (SIRmini_stack.mk cur cont) smo0
+.
+
+Ltac brewrite H := eapply bisim_is_eq; erewrite H; [eapply eq_is_bisim|..].
+(* Tactic Notation "sym" "in" hyp(H) := symmetry in H. *)
+
+Ltac f := first [eapply bisim_is_eq|eapply eq_is_bisim].
+Tactic Notation "f" "in" hyp(H) := first [eapply bisim_is_eq in H|eapply eq_is_bisim in H].
+Ltac ides itr :=
+  let T := fresh "T" in
+  destruct (observe itr) eqn:T;
+  sym in T; apply simpobs in T; apply bisim_is_eq in T; rewrite T in *; clarify.
+
+
+
+
+
+Inductive cont_calls sg fptr oh m0 vs (r0: owned_heap * (mem * val)): list ktr -> nat -> Prop :=
+| cont_calls_now
+    kcall cont_r
+    k_tgt
+    (KCALL: kcall r0 = Vis ((subevent (owned_heap * (mem * val))) (ECall sg fptr oh m0 vs)) k_tgt)
+  :
+    cont_calls sg fptr oh m0 vs r0 (kcall :: cont_r) (0%nat)
+| cont_calls_later
+    kret cont_r r1 n
+    (KRET: kret r0 = Ret r1)
+    (TL: cont_calls sg fptr oh m0 vs r1 cont_r n)
+  :
+    cont_calls sg fptr oh m0 vs r0 (kret :: cont_r) (S n) 
+.
+
+Lemma unfold_cont_call
+      oh sg fptr vs m0
+      (k: ktree (eff0 owned_heap) (owned_heap * (mem * val)) (owned_heap * (mem * val)))
+      (cont: list ktr)
+      (r0: owned_heap * (mem * val))
+      (SIM: Vis (subevent (owned_heap * (mem * val)) (ECall sg fptr oh m0 vs)) k
+                ≅ interp_mrec (interp_function prog) (fold_cont cont r0))
+  :
+    exists n, <<CALLS: cont_calls sg fptr oh m0 vs r0 cont n>>
+.
+Proof.
+  clear - SIM.
+  { ginduction cont; ii; ss.
+    { cbn in SIM. rewrite unfold_interp_mrec in SIM. ss. f in SIM. clarify. }
+    cbn in SIM.
+    (* unfold id_, Id_Kleisli, lift_ktree_ in *. cbn in SIM. ss. *)
+    ides (a r0); autorewrite with itree in SIM.
+    + (* RET *)
+      exploit IHcont; eauto. i; des.
+      exists (S n).
+      econs; eauto.
+    + (* TAU *)
+      rewrite unfold_interp_mrec in SIM. cbn in SIM. f in SIM. clarify.
+    + (* VIS *)
+      rewrite unfold_interp_mrec in SIM. cbn in SIM. f in SIM.
+      des_ifs; clarify; simpl_depind; clarify.
+      esplits; eauto.
+      econs; eauto.
+  }
+Qed.
+
+
+
+
+
+Lemma match_states_lxsim
+      idx st_src0 st_tgt0 smo0
+      (MATCH: match_states idx st_src0 st_tgt0 smo0)
+  :
+    <<XSIM: lxsim (md_src skenv_link) (md_tgt skenv_link)
+                  (fun _ => () -> exists (_ : ()) (_ : mem), True)
+                  (Ord.lift_idx unit_ord_wf idx) st_src0 st_tgt0 smo0>>
+.
+Proof.
+  revert_until idx. revert idx.
+  pcofix CIH. i. pfold.
+  ii. clear SUSTAR.
+
+
+  destruct (classic (ModSem.is_call ms_tgt st_tgt0)).
+  { (*** tgt extcall ***)
+    rr in H. des. ss. inv H. inv MATCH. ss. clarify.
+    econs 3; ss; eauto.
+    { rr. esplits; eauto. ss. econs; eauto.
+      f.
+      rewrite interp_mrec_bind. rewrite unfold_interp_mrec. cbn. autorewrite with itree.
+      f.
+      reflexivity.
+    }
+    ii. clear_tac. inv ATSRC.
+    f in VIS.
+    rewrite interp_mrec_bind in VIS. rewrite unfold_interp_mrec in VIS.
+    cbn in VIS. autorewrite with itree in VIS.
+    f in VIS.
+    clarify; simpl_depind; clarify.
+    inv MWF. ss. destruct smo0; ss. destruct sm0; ss. clarify.
+    eexists _, (Args.mk _ _ _), (mk (SimMemId.mk _ _) _ _); ss. esplits; eauto.
+    { rr. esplits; ss; eauto. econs; ss; eauto. }
+    { econs; ss. }
+    { econs; ss. }
+    ii. clear_tac.
+    inv AFTERSRC. inv GETK. rr in SIMRETV; des; ss.
+    inv SIMRETV0; ss. clarify.
+
+    f in VIS.
+    rewrite interp_mrec_bind in VIS. rewrite unfold_interp_mrec in VIS.
+    cbn in VIS. autorewrite with itree in VIS.
+    f in VIS.
+    clarify; simpl_depind; clarify.
+
+    assert(RMT: forall E R (t: itree E R), Tau t = t).
+    { admit "remove later". }
+
+    esplits; eauto.
+    { econs; eauto. econs; eauto. ss. }
+    right. eapply CIH. econs; ss; eauto.
+    -
+      destruct smo_ret; ss. inv MWF; ss. clarify. destruct sm0; ss. clarify.
+      f.
+      autorewrite with itree.
+      rewrite RMT.
+      rewrite RMT.
+      rewrite interp_mrec_bind.
+      f.
+      ss.
+    - ii.
+      f in RET. autorewrite with itree in RET. f in RET. clarify.
+  }
+  rename H into NCALLTGT.
+
+
+
+  destruct (classic (ModSem.is_return ms_tgt st_tgt0)).
+  { (*** tgt return ***)
+    rr in H. des. ss. inv H. inv MATCH. ss. clarify.
+    econs 4; ss; eauto.
+    { econs; eauto.
+      f.
+      rewrite unfold_interp_mrec. cbn.
+      f.
+      reflexivity.
+    }
+    cbn in SYNC. exploit SYNC; et.
+    { f. rewrite unfold_interp_mrec. cbn. f. reflexivity. }
+    i; des. clarify.
+    inv MWF. rewrite <- OH in *. clarify. destruct smo0; ss. destruct sm0; ss. clarify.
+    rr; ss. esplits; ss; eauto.
+    { econs; ss; eauto. }
+  }
+  rename H into NRETTGT.
+
+
+
+  destruct (classic (ModSem.is_call ms_src st_src0)).
+  {
+    rr in H. des. ss. inv H. inv MATCH. ss.
+    f in SIM.
+    rewrite interp_mrec_bind in SIM. rewrite unfold_interp_mrec in SIM.
+    ides (cur: itree (InternalCallE owned_heap +' EventE owned_heap) _);
+      cbn in SIM; autorewrite with itree in SIM.
+    { (* RET *)
+      exploit unfold_cont_call; eauto. i; des.
+      admit "gogogo with index".
+    }
+    { (* TAU *)
+      f in SIM.
+      clarify.
+    }
+    { (* CALL *)
+      des_ifs.
+      { autorewrite with itree in SIM. f in SIM. clarify. }
+      autorewrite with itree in SIM. f in SIM. clarify; simpl_depind; clarify.
+      econs 3; ss; eauto.
+      { rr. esplits; ss; eauto. econs; ss; eauto. }
+      ii. clear_tac. inv ATSRC; ss.
+      clarify; simpl_depind; clarify.
+      inv MWF. ss. destruct smo0; ss. destruct sm0; ss. clarify.
+      eexists _, (Args.mk _ _ _), (mk (SimMemId.mk _ _) _ _); ss. esplits; eauto.
+      { rr. esplits; ss; eauto. econs; ss; eauto. }
+      { econs; ss. }
+      { econs; ss. }
+      ii. clear_tac.
+      inv AFTERSRC. inv GETK. rr in SIMRETV; des; ss.
+      inv SIMRETV0; ss. clarify; simpl_depind; clarify.
+      assert(RMT: forall E R (t: itree E R), Tau t = t).
+      { admit "remove later". }
+
+      esplits; eauto.
+      { econs; eauto. econs; eauto. ss. }
+      right. eapply CIH. econs; ss; eauto.
+      -
+        destruct smo_ret; ss. inv MWF; ss. clarify. destruct sm0; ss. clarify.
+        f.
+        autorewrite with itree.
+        rewrite RMT.
+        rewrite RMT.
+        rewrite interp_mrec_bind.
+        f.
+        ss.
+      - ii.
+        f in RET. autorewrite with itree in RET. f in RET. clarify.
+    }
+  }
+  rename H into NCALLSRC.
+
+
+
+  destruct (classic (ModSem.is_return ms_src st_src0)).
+  {
+    rr in H. des. ss. inv H. inv MATCH. ss.
+    f in SIM.
+    rewrite interp_mrec_bind in SIM. rewrite unfold_interp_mrec in SIM.
+    ides (cur: itree (InternalCallE owned_heap +' EventE owned_heap) _);
+      cbn in SIM; autorewrite with itree in SIM.
+    { (* RET *)
+      exploit SYNC; eauto. i ;des. clarify.
+      
+    }
+    { (* TAU *)
+      f in SIM.
+      clarify.
+    }
+    { (* CALL *)
+      des_ifs.
+      { autorewrite with itree in SIM. f in SIM. clarify. }
+      autorewrite with itree in SIM. f in SIM. clarify; simpl_depind; clarify.
+      econs 3; ss; eauto.
+      { rr. esplits; ss; eauto. econs; ss; eauto. }
+      ii. clear_tac. inv ATSRC; ss.
+      clarify; simpl_depind; clarify.
+      inv MWF. ss. destruct smo0; ss. destruct sm0; ss. clarify.
+      eexists _, (Args.mk _ _ _), (mk (SimMemId.mk _ _) _ _); ss. esplits; eauto.
+      { rr. esplits; ss; eauto. econs; ss; eauto. }
+      { econs; ss. }
+      { econs; ss. }
+      ii. clear_tac.
+      inv AFTERSRC. inv GETK. rr in SIMRETV; des; ss.
+      inv SIMRETV0; ss. clarify; simpl_depind; clarify.
+      assert(RMT: forall E R (t: itree E R), Tau t = t).
+      { admit "remove later". }
+
+      esplits; eauto.
+      { econs; eauto. econs; eauto. ss. }
+      right. eapply CIH. econs; ss; eauto.
+      -
+        destruct smo_ret; ss. inv MWF; ss. clarify. destruct sm0; ss. clarify.
+        f.
+        autorewrite with itree.
+        rewrite RMT.
+        rewrite RMT.
+        rewrite interp_mrec_bind.
+        f.
+        ss.
+      - ii.
+        f in RET. autorewrite with itree in RET. f in RET. clarify.
+    }
+  }
+
+  assert(NCALLSRC: ~ModSem.is_call ms_src st_src0).
+  {
+    ii. rr in H. des. ss. inv H. inv MATCH. ss.
+    f in SIM.
+    rewrite interp_mrec_bind in SIM. rewrite unfold_interp_mrec in SIM.
+    ides (cur: itree (InternalCallE owned_heap +' EventE owned_heap) _);
+      cbn in SIM; autorewrite with itree in SIM.
+    - contradict NCALLTGT. rr. esplits; ss; et. econs; ss; et.
+  }
+
+
+
+  econs 2; eauto. ii. clear_tac.
+  econs 1; eauto; cycle 1.
+  { ss. exploit SAFESRC; ss; try eapply star_refl; ss. i. des.
+  }
+  - ii. ss. inv STEPTGT; ss.
+Qed.
+
+Theorem sim_modsem: ModSemPair.sim msp.
+Proof.
+  econstructor 1 with (sidx := unit) (sound_states := top4); eauto;
+    try apply sound_state_local_preservation; et; try (by ii; ss).
+  { ii. eapply Preservation.local_preservation_noguarantee_weak.
+    apply sound_state_local_preservation; et.
+  }
+  { ii. ss. eexists (mk _ _ _); ss. esplits; eauto. econs; ss; eauto. }
+  ii. ss. esplits; eauto.
+  - ii. des. esplits; eauto. eapply match_states_lxsim; eauto.
+    admit "".
+  - admit "".
+Qed.
+
+
+
+
+
+
+
+
+
+Theorem sim_modsem: ModSemPair.sim msp.
+Proof.
+  eapply match_states_sim with
+      (match_states := match_states) (match_states_at := top4)
+      (has_footprint := top3) (mle_excl := fun _ _ => SimMemOh.le) (sidx := unit)
+      (order:= bot2);
+    eauto; ii; ss; folder.
+  - eapply SoundTop.sound_state_local_preservation; et.
+  - des. inv INITTGT. inv SAFESRC. ss. des_ifs_safe.
+    rr in SIMARGS. des. ss.  inv SIMARGS0; ss. clarify.
+    assert(fid = fid0).
+    { apply_all_once Genv.find_invert_symbol. clarify. }
+    clarify.
+    esplits; eauto.
+    { econs; eauto. ss. }
+    ss.
+    econs; eauto.
+    + cbn. unfold interp_program0, mrec. cbn.
+      Fail brewrite bind_ret_r. (*** <---- TODO: fix this !!!!!!!!! ***)
+      eapply bisim_is_eq; erewrite bind_ret_r; [eapply eq_is_bisim|..].
+      inv MWF. destruct sm_arg; ss. destruct sm0; ss.
+      rewrite OHSRC0 in *. rewrite OHTGT0 in *. clarify.
+  - des. inv SAFESRC. ss. des_ifs.
+    rr in SIMARGS. des. ss.  inv SIMARGS0; ss. clarify. inv MWF. destruct sm_arg; ss.
+    esplits; eauto.
+    econs; ss; eauto.
+  - inv MATCH. ss.
+  - inv MATCH. ss. inv CALLSRC.
+    eapply eq_is_bisim in VIS; erewrite interp_mrec_bind in VIS; eapply bisim_is_eq in VIS.
+
+    (********* TGT SHOULD TAKE SOME TAU STEPS *********)
+    destruct (observe cur) eqn:T; sym in T; apply simpobs in T; apply bisim_is_eq in T; clarify.
+    { cbn in *.
+      eapply eq_is_bisim in VIS.
+      rewrite unfold_interp_mrec in VIS. cbn in VIS.
+      autorewrite with itree in VIS.
+    }
+      unfold interp_mrec in VIS at 2. cbn in VIS.
+      Erewrite  in VIS; eapply bisim_is_eq in VIS.
+    esplits; eauto.
+    + econs; ss; eauto.
+    
+    exploit eq_itree_inv_vis; eauto.
+    { }
+    destruct (observe (interp_mrec (interp_function prog) cur)) eqn:T.
+    + rewrite itree_eta_ in VIS at 1. cbn in VIS.
+      unfold_bind
+        simpobs
+      rewrite itree_eta in VIS.
+      Set Printing All. rewrite T in VIS.
+    esplits; eauto.
+    + econs; ss; eauto.
+Qed.
 
 End SIMMODSEM.
 
